Give up Knot -- Fib almost works

demo/fib/Fib2.v
@@ -6,8 +6,8 @@ Require Import SmallstepC.
 Require Export Simulation.
 Require Import Skeleton Mod ModSem.
 Require ClightC.
-Require Import FibTarget.
-Require Import SIRmini_quotient.
+Require Import Fib0.
+Require Import SIRmini.
 (* Require Import Clightdefs. *)
 
 Set Implicit Arguments.
@@ -17,7 +17,7 @@ Set Implicit Arguments.
 Definition owned_heap: Type := unit.
 Definition initial_owned_heap: SkEnv.t -> owned_heap := fun _ => tt.
 
-Definition c_fib (oh0: owned_heap) (m0: mem) (vs: list val):
+Definition f_fib (oh0: owned_heap) (m0: mem) (vs: list val):
   itree (E owned_heap) (owned_heap * (mem * val)) :=
   match vs with
   | [Vint n] =>
@@ -30,20 +30,10 @@ Definition c_fib (oh0: owned_heap) (m0: mem) (vs: list val):
         '(oh1, (m1, y1)) <- trigger (ICall _fib oh0 m0 [Vint (Int.sub n (Int.repr 2))]) ;;
         '(oh2, (m2, y2)) <- trigger (ICall _fib oh0 m0 [Vint (Int.sub n (Int.repr 1))]) ;;
         Ret (oh2, (m2, Val.add y1 y2))
-  | _ => triggerUB (owned_heap := owned_heap)
+  | _ => triggerUB
   end
 .
 
-Definition f_fib: function owned_heap :=
-  mkfunction (ClightC.signature_of_function f_fib)
-             (fun oh0 m0 vs => trigger (EBP _) ;; c_fib oh0 m0 vs).
+Definition prog: program owned_heap := (Maps.add _fib f_fib Maps.empty).
 
-Definition global_definitions: list (ident * globdef (fundef (function owned_heap)) unit) :=
-((_fib, Gfun(Internal f_fib)) ::
- nil
-)
-.
-
-Definition prog: program owned_heap := mkprogram global_definitions public_idents _main.
-
-Definition module: Mod.t := module prog "fib"%string initial_owned_heap.
+Definition module: Mod.t := module (Fib0.module) prog "fib"%string initial_owned_heap.
