demo/fib/Fib12proof.v
@@ -1,0 +1,26 @@
+Require Import CoqlibC Maps Postorder.
+Require Import AST Linking.
+Require Import ValuesC MemoryC GlobalenvsC Events Smallstep.
+Require Import Op ClightC.
+Require Import CtypesC CtypingC.
+Require Import sflib.
+Require Import IntegersC.
+
+Require Import Simulation.
+Require Import Skeleton Mod ModSem SimMod SimModSemLift SimSymb SimMemLift MatchSimModSemExcl.
+Require SoundTop.
+Require SimMemId.
+Require Import Any.
+Require Import SIRmini.
+Require Import SIRmini_stack.
+Require Import Fib2.
+Require Import Fib1.
+Require Import ModSemProps.
+Require Import Program.
+Require Import SIRProps.
+
+Set Implicit Arguments.
+
+Definition mp: ModPair.t := SimSymbId.mk_mp (Fib2.module) (Fib1.module).
+Theorem sim_mod: ModPair.sim mp.
+Proof. eapply SIRProps.sim_mod. Qed.
